code/salsa-family/vec256.h
@@ -1,0 +1,91 @@
+#ifndef __Vec_H
+#define __Vec_H
+
+#include <immintrin.h>
+
+#define VEC256
+static const int vec_size = 8;
+
+typedef unsigned int vec256 __attribute__ ((vector_size (32)));
+
+typedef struct {
+  vec256 v;
+} vec;
+
+static inline vec vec_load_32x4(uint32_t x1, uint32_t x2, uint32_t x3, uint32_t x4){
+  vec v;
+  v.v = (vec256) {x1,x2,x3,x4,x1,x2,x3,x4};
+  return v;
+}
+
+
+static inline vec vec_load_32x8(uint32_t x1, uint32_t x2, uint32_t x3, uint32_t x4, uint32_t x5, uint32_t x6, uint32_t x7, uint32_t x8){
+  vec v;
+  v.v = (vec256) {x1,x2,x3,x4,x5,x6,x7,x8};
+  return v;
+}
+
+
+static inline vec vec_rotate_left(vec v, unsigned int n) {
+  vec r;
+  r.v = (vec256)((v.v << n) ^ (v.v >> (32-n)));
+  return r;
+}
+
+static inline vec vec_rotate_right(vec v, unsigned int n) {
+  return (vec_rotate_left(v,32-n));
+}
+
+static inline vec vec_shuffle_right(vec x, unsigned int n) {
+  vec r;
+  r.v = ((vec256)_mm256_shuffle_epi32((__m256i)x.v,_MM_SHUFFLE((3+n)%4,(2+n)%4,(1+n)%4,n%4)));
+  return r;
+}
+
+static inline vec vec_shuffle_left(vec x, unsigned int n) {
+  return (vec_shuffle_right(x,4-n));
+}
+
+static inline vec vec_load_le(const unsigned char* in) {
+  vec r;
+  r.v = (vec256) _mm256_loadu_si256((__m256i*)(in));
+  return r;
+}
+
+static inline void vec_store_le(unsigned char* out, vec v) {
+  _mm256_storeu_si256((__m256i*)(out), (__m256i) v.v);
+}
+
+
+static inline vec vec_load128_le(const unsigned char* in) {
+  vec r;
+  __m128i x = _mm_loadu_si128((__m128i*)(in));
+  r.v = (vec256) _mm256_broadcastsi128_si256 (x);
+  return r;
+}
+
+
+static inline vec vec_add(vec v1, vec v2) {
+  vec r;
+  r.v = (vec256) v1.v + v2.v;
+  return r;
+}
+
+static inline vec vec_xor(vec v1, vec v2) {
+  vec r;
+  r.v = (vec256)v1.v ^ v2.v;
+  return r;
+}
+
+static const vec two_le = {.v = {2,0,0,0,2,0,0,0}};
+static const vec one_le = {.v = {1,0,0,0,1,0,0,0}};
+static const vec zero = {.v = {0,0,0,0,0,0,0}};
+
+static inline vec vec_choose_128(vec v1, vec v2, unsigned int first, unsigned int second) {
+  vec r;
+  unsigned char control = (second * 16) + first;
+  r.v = (vec256)_mm256_permute2x128_si256((__m256i)v1.v, (__m256i)v2.v, control);
+  return r;
+}
+
+#endif
